\documentclass[11pt]{article}
\usepackage{thesis}

\begin{document}
\section{Introduction}
This is the equation for logistic map:
\begin{equation}
  L_{\mu}(x) = \mu x(1-x)
  \label{logistic}
\end{equation}
, and the ``equivalent'' differential equation:
\begin{equation}
  \frac{dx}{dt} = \mu x(1-x)
  \label{logisticdiffeq}
\end{equation}
This can be solved by separation of variables.
\begin{align*}
  \frac{dx}{x(1-x)} &= \mu dt \\  
  \left( \frac{1}{x} + \frac{1}{1-x} \right) dx &= \mu dt
\end{align*}
Then, suppose that $x(0) = x_0$, and integrate from $t = 0$ to $T$
\begin{align*}
  \int_{x_0}^{x(T)} \frac{1}{x} + \frac{1}{1-x} dx &= \int_0^T \mu dt \\
  \log{\frac{x(T)}{1-x(T)}} - \log{\frac{x_0}{1-x_0}} &= \mu T \\
  \frac{x(T)}{1-x(T)} &= \frac{x_0 e^{\mu T}}{1-x_0} \\
  (1-x_0)x(T) &= x_0 e^{\mu T} (1-x(T))
  (1-x_0 + x_0 e^{\mu T})x(T) &= x_0 e^{\mu T}
\end{align*}

Thus, we have (with a slight change of notation)
\begin{equation}
  x(t) = \frac{x_0 e^{\mu t}}{1 - x_0 + x_0 e^{\mu t}}
  \label{logisticdiffeqsoln}
\end{equation}


\end{document}
